CBPV/Normalization.lean
@@ -30,20 +30,22 @@ theorem NeCom.ne {m} (snem : SNeCom m) : NeCom m := by
 joint
   theorem SNeCom.SN_soundness {m} (sne : SNeCom m) : StepCom.SN m
   theorem SNVal.SN_soundness {v} (sn : SNVal v) : StepVal.SN v
-  theorem SNCom.SN_soundness {m} (sn : SNCom  m) : StepCom.SN m
-  theorem Sr.SN_soundness {m n : Com} (r : m ⤳ n) : m ⤳ⁿ n
+  theorem SNCom.SN_soundness {m} (sn : SNCom m) : StepCom.SN m
+  theorem SR.SN_soundness {m n : Com} (r : m ⤳ n) : m ⤳ⁿ n
 by
   mutual_induction sne, sn, sn, r
   case force snv => exact .force snv
   case app snem _ snm snv => exact .app (.ne snem) snm snv
   case letin snem _ snm snn => exact .letin (.ne snem) snm snn
   case case snv _ _ snm snn => exact .case snv snm snn
+  case unpair snev _ snm => exact .unpair snev snm
   case fst snem snm => exact .fst (.ne snem) snm
   case snd snem snm => exact .snd (.ne snem) snm
   case var => constructor; intro _ r; cases r
   case unit => constructor; intro _ r; cases r
   case inl ih => exact .inl ih
   case inr ih => exact .inr ih
+  case pair ihv ihw => exact .pair ihv ihw
   case thunk ih => exact .thunk ih
   case lam ih => exact .lam ih
   case ret ih => exact .ret ih
