CBPV/Typing.lean
@@ -22,6 +22,11 @@ inductive ValWt : Ctxt → Val → ValType → Prop where
     Γ ⊢ v ∶ A₂ →
     ---------------------
     Γ ⊢ inr v ∶ Sum A₁ A₂
+  | pair {Γ v w} {A₁ A₂ : ValType} :
+    Γ ⊢ v ∶ A₁ →
+    Γ ⊢ w ∶ A₂ →
+    -------------------------
+    Γ ⊢ pair v w ∶ Pair A₁ A₂
   | thunk {Γ m} {B : ComType} :
     Γ ⊢ m ∶ B →
     -----------------
@@ -56,6 +61,11 @@ inductive ComWt : Ctxt → Com → ComType → Prop where
     Γ ∷ A₂ ⊢ n ∶ B →
     ------------------
     Γ ⊢ case v m n ∶ B
+  | unpair {Γ v m A₁ A₂} {B : ComType} :
+    Γ ⊢ v ∶ Pair A₁ A₂ →
+    Γ ∷ A₁ ∷ A₂ ⊢ m ∶ B →
+    ------------------
+    Γ ⊢ unpair v m ∶ B
   | prod {Γ m n} {B₁ B₂: ComType} :
     Γ ⊢ m ∶ B₁ →
     Γ ⊢ n ∶ B₂ →
@@ -97,37 +107,3 @@ theorem wtWeakenCom {Γ A B} {m : Com} :
 theorem wtWeakenCom₂ {Γ A₁ A₂ B} {m : Com} :
   Γ ∷ A₂ ⊢ m ∶ B → Γ ∷ A₁ ∷ A₂ ⊢ renameCom (lift succ) m ∶ B :=
   wtRenameCom (wRenameLift wRenameSucc)
-
-/-*--------------------------------------
-  Rearrangement lemmas for commutations
---------------------------------------*-/
-
-theorem wtLetApp {Γ n m v A B} (hlet : Γ ⊢ letin n m ∶ Arr A B) (hv : Γ ⊢ v ∶ A) :
-  Γ ⊢ letin n (app m (renameVal succ v)) ∶ B := by
-  cases hlet with | letin hn hm =>
-  exact .letin hn (.app hm (wtWeakenVal hv))
-
-theorem wtLetFst {Γ n m B₁ B₂} (hlet : Γ ⊢ letin n m ∶ Prod B₁ B₂) :
-  Γ ⊢ letin n (fst m) ∶ B₁ := by
-  cases hlet with | letin hn hm =>
-  exact .letin hn (.fst hm)
-
-theorem wtLetSnd {Γ n m B₁ B₂} (hlet : Γ ⊢ letin n m ∶ Prod B₁ B₂) :
-  Γ ⊢ letin n (snd m) ∶ B₂ := by
-  cases hlet with | letin hn hm =>
-  exact .letin hn (.snd hm)
-
-theorem wtCaseApp {Γ v m₁ m₂ w A B} (hcase : Γ ⊢ case v m₁ m₂ ∶ Arr A B) (hw : Γ ⊢ w ∶ A) :
-  Γ ⊢ case v (app m₁ (renameVal succ w)) (app m₂ (renameVal succ w)) ∶ B := by
-  cases hcase with | case hv hm₁ hm₂ =>
-  exact .case hv (.app hm₁ (wtWeakenVal hw)) (.app hm₂ (wtWeakenVal hw))
-
-theorem wtCaseFst {Γ v m₁ m₂ B₁ B₂} (hcase : Γ ⊢ case v m₁ m₂ ∶ Prod B₁ B₂) :
-  Γ ⊢ case v (fst m₁) (fst m₂) ∶ B₁ := by
-  cases hcase with | case hv hm₁ hm₂ =>
-  exact .case hv (.fst hm₁) (.fst hm₂)
-
-theorem wtCaseSnd {Γ v m₁ m₂ B₁ B₂} (hcase : Γ ⊢ case v m₁ m₂ ∶ Prod B₁ B₂) :
-  Γ ⊢ case v (snd m₁) (snd m₂) ∶ B₂ := by
-  cases hcase with | case hv hm₁ hm₂ =>
-  exact .case hv (.snd hm₁) (.snd hm₂)
